crypto/bignum/poly1305/Hacl.Spec.MAC.Poly1305_64.fst
@@ -26,7 +26,7 @@ let elem : Type0 = b:int{ b >= 0 /\ b < prime }
 let word = b:Seq.seq H8.t{Seq.length b <= 16}
 let word_16 = b:Seq.seq H8.t{Seq.length b = 16}
 
-(* noeq type poly1305_state_ = | MkState: r:seqelem -> h:seqelem -> poly1305_state_ *)
+noeq type poly1305_state_ = | MkState: r:seqelem -> h:seqelem -> log:log_t -> poly1305_state_
 
 #reset-options "--initial_fuel 0 --max_fuel 0 --z3rlimit 20"
 
@@ -155,61 +155,61 @@ let toField_plus_2_128_spec m =
   Seq.upd b 2 b2'
 
 
+(* #reset-options "--initial_fuel 0 --max_fuel 0 --z3rlimit 20" *)
+
+(* assume val lemma_logor_max: #n:pos -> a:UInt.uint_t n -> b:UInt.uint_t n -> m:nat{m <= n} -> Lemma *)
+(*   (requires (a < pow2 m /\ b < pow2 m)) *)
+(*   (ensures (UInt.logor a b < pow2 m)) *)
+
+(* val toField_plus_spec: len:U32.t{U32.v len < 16} -> m:word{Seq.length m = U32.v len} -> *)
+(*   Tot (s:seqelem{red_44 s}) *)
+(* let toField_plus_spec len m' = *)
+(*   cut (pow2 (24 + U32.v len) % pow2 (24 + U32.v len) = 0); *)
+(*   let m = Seq.append m' (Seq.create (16 - U32.v len) (uint8_to_sint8 0uy)) in *)
+(*   let b = toField_spec m in *)
+(*   let b2 = Seq.index b 2 in *)
+(*   let open Hacl.Bignum.Limb in *)
+(*   let b2' = uint64_to_sint64 1uL <<^ (U32.(24ul +^ len)) |^ b2 in *)
+(*   Math.Lemmas.pow2_lt_compat 64 (24 + U32.v len); *)
+(*   Math.Lemmas.modulo_lemma (pow2 (24 + U32.v len)) (pow2 64); *)
+(*   Math.Lemmas.pow2_lt_compat 44 (24 + U32.v len); *)
+(*   lemma_logor_max #64 (pow2 (24 + U32.v len)) (v b2) 44; *)
+(*   Seq.upd b 2 b2' *)
+
+
+(* #reset-options "--initial_fuel 0 --max_fuel 0 --z3rlimit 20" *)
+
+(* val poly1305_finish_spec: acc:seqelem{red_45 acc} -> key_s:Seq.seq H8.t{Seq.length key_s = 16} -> *)
+(*   Tot (mac:Seq.seq H8.t{Seq.length mac = 16}) *)
+(* let poly1305_finish_spec acc key_s = *)
+(*   Math.Lemmas.pow2_lt_compat 63 44; *)
+(*   let acc1 = Hacl.Spec.Bignum.Fproduct.carry_limb_spec acc 0 in *)
+(*   (\* assume (v (Seq.index (as_seq h1 acc) 2) < pow2 45 + pow2 20); *\) *)
+(*   assert_norm(pow2 45 + pow2 20 = 0x200000000000 + 0x100000); *)
+(*   assert_norm(pow2 42 = 0x40000000000); *)
+(*   assert_norm(pow2 44 = 0x100000000000); *)
+(*   assert_norm(pow2 64 = 0x10000000000000000); *)
+(*   let acc2 = Hacl.Spec.Bignum.Modulo.carry_top_spec acc1 in *)
+(*   let acc3 = Hacl.Spec.Bignum.Fproduct.carry_0_to_1_spec acc in *)
+(*   (\* Adding 2nd part of the key (one time pad) *\) *)
+(*   let key = toField_spec key_s in *)
+(*   let acc4 = Hacl.Spec.Bignum.Fsum.fsum_spec acc key len in *)
+(*   (\* Last carry and truncation *\) *)
+(*   let acc5 = Hacl.Spec.Bignum.Fproduct.carry_limb_spec acc 0 in *)
+(*   let h0 = Seq.index acc5 0 in *)
+(*   let h1 = Seq.index acc5 1 in *)
+(*   let h2 = Seq.index acc5 2 in *)
+(*   let open Hacl.Bignum.Limb in *)
+(*   let h0 = h0 |^ (h1 <<^ 44ul) in *)
+(*   let h1 = (h1 >>^ 20ul) |^ (h2 <<^ 24ul) in *)
+(*   let mac0 = store64_le_spec h0 in *)
+(*   let mac1 = store64_le_spec h1 in *)
+(*   Seq.append mac0 mac1 *)
+
+
 #reset-options "--initial_fuel 0 --max_fuel 0 --z3rlimit 20"
 
-assume val lemma_logor_max: #n:pos -> a:UInt.uint_t n -> b:UInt.uint_t n -> m:nat{m <= n} -> Lemma
-  (requires (a < pow2 m /\ b < pow2 m))
-  (ensures (UInt.logor a b < pow2 m))
-
-val toField_plus_spec: len:U32.t{U32.v len < 16} -> m:word{Seq.length m = U32.v len} ->
-  Tot (s:seqelem{red_44 s})
-let toField_plus_spec len m' =
-  cut (pow2 (24 + U32.v len) % pow2 (24 + U32.v len) = 0);
-  let m = Seq.append m' (Seq.create (16 - U32.v len) (uint8_to_sint8 0uy)) in
-  let b = toField_spec m in
-  let b2 = Seq.index b 2 in
-  let open Hacl.Bignum.Limb in
-  let b2' = uint64_to_sint64 1uL <<^ (U32.(24ul +^ len)) |^ b2 in
-  Math.Lemmas.pow2_lt_compat 64 (24 + U32.v len);
-  Math.Lemmas.modulo_lemma (pow2 (24 + U32.v len)) (pow2 64);
-  Math.Lemmas.pow2_lt_compat 44 (24 + U32.v len);
-  lemma_logor_max #64 (pow2 (24 + U32.v len)) (v b2) 44;
-  Seq.upd b 2 b2'
-
-
-#reset-options "--initial_fuel 0 --max_fuel 0 --z3rlimit 20"
-
-val poly1305_finish_spec: acc:seqelem{red_45 acc} -> key_s:Seq.seq H8.t{Seq.length key_s = 16} ->
-  Tot (mac:Seq.seq H8.t{Seq.length mac = 16})
-let poly1305_finish_spec acc key_s =
-  Math.Lemmas.pow2_lt_compat 63 44;
-  let acc1 = Hacl.Spec.Bignum.Fproduct.carry_limb_spec acc 0 in
-  (* assume (v (Seq.index (as_seq h1 acc) 2) < pow2 45 + pow2 20); *)
-  assert_norm(pow2 45 + pow2 20 = 0x200000000000 + 0x100000);
-  assert_norm(pow2 42 = 0x40000000000);
-  assert_norm(pow2 44 = 0x100000000000);
-  assert_norm(pow2 64 = 0x10000000000000000);
-  let acc2 = Hacl.Spec.Bignum.Modulo.carry_top_spec acc1 in
-  let acc3 = Hacl.Spec.Bignum.Fproduct.carry_0_to_1_spec acc in
-  (* Adding 2nd part of the key (one time pad) *)
-  let key = toField_spec key_s in
-  let acc4 = Hacl.Spec.Bignum.Fsum.fsum_spec acc key len in
-  (* Last carry and truncation *)
-  let acc5 = Hacl.Spec.Bignum.Fproduct.carry_limb_spec acc 0 in
-  let h0 = Seq.index acc5 0 in
-  let h1 = Seq.index acc5 1 in
-  let h2 = Seq.index acc5 2 in
-  let open Hacl.Bignum.Limb in
-  let h0 = h0 |^ (h1 <<^ 44ul) in
-  let h1 = (h1 >>^ 20ul) |^ (h2 <<^ 24ul) in
-  let mac0 = store64_le_spec h0 in
-  let mac1 = store64_le_spec h1 in
-  Seq.append mac0 mac1
-
-
-#reset-options "--initial_fuel 0 --max_fuel 0 --z3rlimit 20"
-
-val poly1305_start_spec: unit -> Tot (s:seqelem{Seq.index s 0 == limb_zero /\ Seq.index s 1 == limb_zero /\ Seq.index s 2 == limb_zero /\ selem s = 0})
+val poly1305_start_spec: unit -> Tot (s:seqelem{Seq.index s 0 == limb_zero /\ Seq.index s 1 == limb_zero /\ Seq.index s 2 == limb_zero /\ selem s = 0 /\ red_45 s})
 let poly1305_start_spec () =
   let s = Seq.create len limb_zero in
   lemma_seval_def (s) 3;
@@ -218,157 +218,107 @@ let poly1305_start_spec () =
   lemma_seval_def (s) 0;
   s
 
+
 #reset-options "--initial_fuel 0 --max_fuel 0 --z3rlimit 20"
 
-
-(* ******************* *)
-(* Fast implementation *)
-(* ******************* *)
-
-
-val poly1305_init_:
-  st:poly1305_state ->
-  key:uint8_p{length key = 32} ->
-  Stack log_t
-    (requires (fun h -> live_st h st /\ live h key /\ red_45 (as_seq h st.h) /\ disjoint st.r key
-      /\ disjoint st.h key))
-    (ensures  (fun h0 log h1 -> modifies_2 st.r st.h h0 h1
-      /\ live h1 st.r /\ live h1 st.h /\ red_44 (as_seq h1 st.r) /\ red_45 (as_seq h1 st.h)
-      ))
-let poly1305_init_ st key =
-  poly1305_encode_r st.r (sub key 0ul 16ul);
-  poly1305_start st.h
+val poly1305_init_spec: key:Seq.seq H8.t{Seq.length key = 32} ->
+  Tot (st:poly1305_state_{red_44 (MkState?.r st) /\ red_45 (MkState?.h st)})
+let poly1305_init_spec key =
+  let r = poly1305_encode_r_spec (Seq.slice key 0 16) in
+  let h = poly1305_start_spec () in
+  MkState r h ()
 
 
-val poly1305_update:
-  current_log:log_t ->
-  st:poly1305_state ->
-  m:uint8_p{length m >= 16} ->
-  Stack log_t
-    (requires (fun h -> live_st h st /\ live h m /\ disjoint m st.h /\ disjoint m st.r
-      /\ red_45 (as_seq h st.h)
-      /\ red_44 (as_seq h st.r)
-      (* /\ acc_inv h current_log st *)
-      ))
-    (ensures  (fun h0 updated_log h1 -> modifies_1 st.h h0 h1 /\ live_st h1 st
-      /\ red_45 (as_seq h1 st.h)
-      (* /\ acc_inv h1 updated_log st *)
-      (* /\ (reveal updated_log) == *)
-      (*     SeqProperties.snoc (reveal current_log) (encode (sel_word h1 (Buffer.sub m 0ul 16ul))) *)
-      (* /\ sel_elem h1 st.h == poly (reveal updated_log) (sel_elem h0 st.r) *)
-      ))
-let poly1305_update log st m =
-  push_frame();
-  let tmp = create limb_zero clen in
-  let acc = st.h in
-  let r   = st.r in
-  toField_plus_2_128 tmp (sub m 0ul 16ul);
-  add_and_multiply acc tmp r;
-  let new_log = (* elift1 (fun l -> SeqProperties.snoc l (eval_3_limbs h0 h1 h2)) log in *) () in
-  pop_frame();
-  new_log
+val poly1305_update_spec: st:poly1305_state_{red_44 (MkState?.r st) /\ red_45 (MkState?.h st)} ->
+  m:Seq.seq H8.t{Seq.length m >= 16} ->
+  Tot (st':poly1305_state_{red_44 (MkState?.r st') /\ red_45 (MkState?.h st')})
+let poly1305_update_spec st m =
+  let block = toField_plus_2_128_spec (Seq.slice m 0 16) in
+  let acc = MkState?.h st in
+  let r = MkState?.r st in
+  let log = MkState?.log st in
+  let acc' = add_and_multiply_tot acc block r in
+  MkState r acc' log
 
 
-val poly1305_blocks:
-  current_log:log_t ->
-  st:poly1305_state ->
-  m:uint8_p ->
-  len:U64.t{U64.v len <= length m} ->
-  Stack log_t
-    (requires (fun h -> live_st h st /\ live h m /\ disjoint st.r m /\ disjoint st.h m
-      /\ red_45 (as_seq h st.h)
-      /\ red_44 (as_seq h st.r)
-      (* /\ acc_inv h current_log st *)
-      ))
-    (ensures  (fun h0 updated_log h1 -> modifies_1 st.h h0 h1 /\ live_st h1 st
-      /\ red_45 (as_seq h1 st.h)
-      (* /\ acc_inv h1 updated_log st *)
-      (* /\ (reveal updated_log) == *)
-      (*     encode_pad (reveal current_log) (as_seq h0 (Buffer.sub m 0ul (Int.Cast.uint64_to_uint32 len))) *)
-      (* /\ sel_elem h1 st.h == poly (reveal updated_log) (sel_elem h0 st.r) *)
-      ))
-let rec poly1305_blocks log st m len =
-  let m0 = ST.get() in
-  if U64.(len <^ 16uL) then (
-    (* log *)
-    ()
-  )
+val poly1305_blocks_spec: st:poly1305_state_{red_44 (MkState?.r st) /\ red_45 (MkState?.h st)} ->
+  m:Seq.seq H8.t ->
+  len:U64.t{U64.v len <= Seq.length m} -> 
+  Tot (st':poly1305_state_{red_44 (MkState?.r st') /\ red_45 (MkState?.h st')})
+  (decreases (U64.v len))
+let rec poly1305_blocks_spec st m len =
+  if U64.(len <^ 16uL) then st
   else (
-    let new_log = poly1305_update log st m in
+    let st' = poly1305_update_spec st m in
     let len = U64.(len -^ 16uL) in
-    let m   = offset m 16ul in
-    poly1305_blocks new_log st m len
+    let m'   = Seq.slice m 16 (Seq.length m) in
+    poly1305_blocks_spec st' m' len
   )
 
 
-val poly1305_finish_:
-  log:log_t ->
-  st:poly1305_state ->
-  mac:uint8_p ->
-  m:uint8_p ->
-  len:U64.t{U64.v len < pow2 32 /\ U64.v len <= length m} ->
-  key_s:uint8_p{length key_s = 16} ->
-  Stack log_t
-    (requires (fun h -> (* acc_inv h log st *)live_st h st /\ live h mac /\ live h m /\ live h key_s
-      /\ disjoint st.h mac
-      /\ red_44 (as_seq h st.r) /\ red_45 (as_seq h st.h)))
-    (ensures  (fun h0 updated_log h1 -> modifies_2 st.h mac h0 h1
-      /\ live h1 st.h /\ live h1 mac
-      (* /\ acc_inv h1 updated_log st *)
-      ))
-let poly1305_finish_ log st mac m len key_s =
-  push_frame();
-  let tmp   = create limb_zero clen in
+
+val poly1305_process_last_block_spec:
+  st:poly1305_state_{red_44 (MkState?.r st) /\ red_45 (MkState?.h st)} ->
+  m:Seq.seq H8.t ->
+  rem':U64.t{U64.v rem' = Seq.length m /\ U64.v rem' < 16} ->
+  Tot (st':poly1305_state_{red_44 (MkState?.r st') /\ red_45 (MkState?.h st')})
+let poly1305_process_last_block_spec st m rem' =
+  let m' = Seq.append m (Seq.create (16 - U64.v rem') (uint8_to_sint8 0uy)) in
+  let m'' = Seq.upd m' (U64.v rem') (uint8_to_sint8 1uy) in
+  let block = toField_spec m'' in
+  let acc = MkState?.h st in
+  let r = MkState?.r st in
+  let log = MkState?.log st in
+  let acc' = add_and_multiply_tot acc block r in
+  MkState r acc' log
+
+
+#set-options "--lax"
+
+val poly1305_last_pass_spec: acc:seqelem{red_45 acc} -> Tot (acc':seqelem)
+let poly1305_last_pass_spec acc =
+  let acc1 = Hacl.Spec.Bignum.Fproduct.carry_limb_spec acc 0 in
+  let acc2 = Hacl.Spec.Bignum.Modulo.carry_top_spec acc1 in
+  Hacl.Spec.Bignum.Fproduct.carry_0_to_1_spec acc2
+
+
+#reset-options "--initial_fuel 0 --max_fuel 0 --z3rlimit 50"
+
+val poly1305_finish_spec: st:poly1305_state_{red_44 (MkState?.r st) /\ red_45 (MkState?.h st)} ->
+  m:Seq.seq H8.t ->
+  len:U64.t{U64.v len < pow2 32 /\ U64.v len <= Seq.length m} ->
+  key_s:Seq.seq H8.t{Seq.length key_s = 16} ->
+  Tot (m:Seq.seq H8.t{Seq.length m = 16})
+let poly1305_finish_spec st m len key_s =
   let rem' = U64.(len &^ 0xfuL) in
   assert_norm(pow2 4 - 1 = 0xf);
   UInt.logand_mask (U64.v len) 4;
-  if U64.(rem' =^ 0uL) then ()
-  else (
-    let zero = uint8_to_sint8 0uy in
-    let block = create zero 16ul in
-    let i = FStar.Int.Cast.uint64_to_uint32 rem' in
-    Math.Lemmas.modulo_lemma (U64.v len - U64.v rem') (pow2 32);
-    blit m (FStar.Int.Cast.uint64_to_uint32 (U64.(len -^ rem'))) block 0ul i;
-    block.(i) <- uint8_to_sint8 1uy;
-    toField tmp block;
-    add_and_multiply st.h tmp st.r
-    );
-  Hacl.Bignum.Fproduct.carry_limb_ st.h 0ul;
-  Hacl.Bignum.Modulo.carry_top st.h;
-  Hacl.Bignum.Fproduct.carry_0_to_1 st.h;
-  toField tmp key_s;
-  Hacl.Bignum.Fsum.fsum_ st.h tmp clen;
-  Hacl.Bignum.Fproduct.carry_limb_ st.h 0ul;
-  let h0 = st.h.(0ul) in
-  let h1 = st.h.(1ul) in
-  let h2 = st.h.(2ul) in
+  let st' = if U64.(rem' =^ 0uL) then st
+           else poly1305_process_last_block_spec st (Seq.slice m 0 (U64.v rem')) rem' in
+  let acc = poly1305_last_pass_spec (MkState?.h st') in
+  let kl = load64_le_spec (Seq.slice key_s 0 8) in
+  let kh = load64_le_spec (Seq.slice key_s 8 16) in
+  let h0 = Seq.index acc 0 in
+  let h1 = Seq.index acc 1 in
+  let h2 = Seq.index acc 2 in
   let open Hacl.Bignum.Limb in
-  let h0 = h0 |^ (h1 <<^ 44ul) in
-  let h1 = (h1 >>^ 20ul) |^ ((h2 &^ mask_42) <<^ 24ul) in
-  store64_le mac h0;
-  store64_le (offset mac 8ul) h1;
-  pop_frame();
-  log // TODO
+  let accl = h0 |^ (h1 <<^ 44ul) in
+  let acch = (h1 >>^ 20ul) |^ (h2 <<^ 24ul) in
+  let open Hacl.Bignum.Wide in
+  let acc' = limb_to_wide accl |^ (limb_to_wide acch <<^ 64ul) in
+  let k'   = limb_to_wide kl   |^ (limb_to_wide kh   <<^ 64ul) in
+  let mac = acc' +%^ k' in
+  let macl = wide_to_limb mac in
+  let mach = wide_to_limb (mac >>^ 64ul) in
+  Seq.append (store64_le_spec macl) (store64_le_spec mach)
 
 
-val crypto_onetimeauth:
-  output:uint8_p ->
-  input:uint8_p ->
-  len:U64.t ->
-  k:uint8_p ->
-  Stack unit
-    (requires (fun _ -> True))
-    (ensures  (fun _ _ _ -> True))
-let crypto_onetimeauth output input len k =
-  push_frame();
-  let zero = uint64_to_sint64 0uL in
-  let r = create zero clen in
-  let h = create zero clen in
-  let st = MkState r h in
-  (* let st = {r = r; h = h} in *)
-  let key_r = Buffer.sub k 0ul 16ul in
-  let key_s = Buffer.sub k 16ul 16ul in
-  let init_log = poly1305_init_ st key_r in
-  let partial_log = poly1305_blocks init_log st input len in
-  let final_log = poly1305_finish_ partial_log st output input len key_s in
-  pop_frame()
+val crypto_onetimeauth_spec:
+  input:Seq.seq H8.t ->
+  len:U64.t{U64.v len < pow2 32 /\ U64.v len < Seq.length input} ->
+  k:Seq.seq H8.t{Seq.length k = 32} ->
+  Tot (mac:Seq.seq H8.t{Seq.length mac = 16})
+let crypto_onetimeauth_spec input len k =
+  let init_st = poly1305_init_spec k in  
+  let partial_st = poly1305_blocks_spec init_st input len in
+  poly1305_finish_spec partial_st input len (Seq.slice k 16 32)
